WAS lock

theories/waslock.v
@@ -1,21 +1,51 @@
-From diris.heap_lang Require Export proofmode notation.
-Set Default Proof Using "Type".
+From iris.base_logic.lib Require Import invariants.
+From diris.heap_lang Require Import proofmode notation.
 
 Definition newlock : val := λ: <>, ref #false.
-Definition lock : val := λ: "x", WAS "x" #false #true.
-Definition unlock : val := λ: "x", "x" <- #true.
+Definition acquire : val := λ: "l", WAS "l" #false #true.
+Definition release : val := λ: "l", "l" <- #false.
 
 Section proof.
   Context `{!heapG Σ}.
 
-  Lemma foo x a : vals_compare_safe a #false → {{{ x ↦ a }}} lock #x {{{ RET #(); x ↦ #true }}}.
+  Definition lock_inv (l : loc) (R : iProp Σ) : iProp Σ :=
+    (∃ b : bool, l ↦ #b ∗ if b then True else R)%I.
+
+  Definition lockN : namespace := nroot .@ "lock".
+  Definition is_lock (lk : val) (R : iProp Σ) : iProp Σ :=
+    (∃ l: loc, ⌜ lk = #l ⌝ ∧ inv lockN (lock_inv l R))%I.
+
+  Lemma newlock_spec (R : iProp Σ):
+    {{{ R }}} newlock #() {{{ lk, RET lk; is_lock lk R }}}.
   Proof.
-    intros Hvcs.
-    iIntros (Φ) "Hx Post".
+    iIntros (Φ) "HR HΦ". iApply wp_fupd.
+    wp_lam. wp_alloc l as "Hl".
+    iMod (inv_alloc lockN _ (lock_inv l R) with "[HR Hl]") as "#Hinv".
+    { iNext. iExists false. iFrame. }
+    iModIntro. iApply "HΦ". iExists l. eauto.
+  Qed.
+
+  Lemma acquire_spec lk R :
+    {{{ is_lock lk R }}} acquire lk {{{ RET #(); R }}}.
+  Proof.
+    iIntros (Φ) "#Hl HΦ". iDestruct "Hl" as (l ->) "#Hinv".
     wp_lam.
-    Check wp_was.
-    wp_apply (wp_was with "Hx").
-    - done.
-    - iIntros "H". iApply "Post". iDestruct "H" as "[H1 H2]". iFrame.
+    iInv lockN as (b) "[Hl HR]" "Hclose".
+    wp_apply (wp_was with "Hl").
+    - naive_solver.
+    - iIntros "[% Hl]". iMod ("Hclose" with "[Hl]") as "_".
+      { iNext. iExists true. iFrame. }
+      iApply "HΦ". simplify_eq. iModIntro. iFrame.
+  Qed.
+
+  Lemma release_spec lk R :
+    {{{ is_lock lk R ∗ R }}} release lk {{{ RET #(); True }}}.
+  Proof.
+    iIntros (Φ) "[#Hl HR] Post".
+    wp_lam. iDestruct "Hl" as (l) "[-> Hinv]".
+    iInv lockN as (b) "[Hl _]" "Hclose".
+    wp_store. iMod ("Hclose" with "[Hl HR]") as "_".
+    - iNext. iExists false. iFrame.
+    - iApply "Post". done. 
   Qed.
 End proof.
