theories/spinlock.v
@@ -101,8 +101,13 @@ Section proof.
     destruct b.
     - wp_cmpxchg_fail. iMod ("Hclose" with "[Hl]") as "_".
       { iNext. iExists true. iFrame. }
-      iModIntro. wp_proj. (* exercise *)
-  Admitted.
+      iModIntro. wp_proj.
+      iApply "HΦ". done.
+    - wp_cmpxchg_suc. iMod ("Hclose" with "[Hl]") as "_".
+      { iNext. iExists true. iFrame. }
+      iModIntro. wp_proj.
+      iApply "HΦ". done.
+  Qed.
 
   (** *Exercise*: prove the spec of [acquire]. Since [acquire] is a recursive
   function, you should use the tactic [iLöb] for Löb induction. Use the tactic
@@ -110,8 +115,13 @@ Section proof.
   Lemma acquire_spec lk R :
     {{{ is_lock lk R }}} acquire lk {{{ RET #(); R }}}.
   Proof.
-    (* exercise *)
-  Admitted.
+    iIntros (Φ) "#Hl Post".
+    iLöb as "IH".
+    wp_rec. wp_apply (try_acquire_spec with "Hl").
+    iIntros ([]) "Hb".
+    - wp_pures. iApply "Post". iFrame.
+    - wp_pures. iApply "IH". iNext. iApply "Post".
+  Qed.  
 
   (** *Exercise*: prove the spec of [release]. At a certain point in this proof,
   you need to open the invariant. For this you can use:
@@ -123,6 +133,11 @@ Section proof.
   Lemma release_spec lk R :
     {{{ is_lock lk R ∗ R }}} release lk {{{ RET #(); True }}}.
   Proof.
-    (* exercise *)
-  Admitted.
+    iIntros (Φ) "[#Hl HR] Post".
+    wp_lam. iDestruct "Hl" as (l) "[-> Hinv]".
+    iInv lockN as (b) "[Hl _]" "Hclose".
+    wp_store. iMod ("Hclose" with "[Hl HR]") as "_".
+    - iNext. iExists false. iFrame.
+    - iApply "Post". done. 
+  Qed.
 End proof.
